WIP

PDDL-sema/Terms.thy
@@ -2,26 +2,26 @@ theory Terms
   imports AST1
 begin
 
-  type_synonym 'sym function_interpretation = "'sym term \<rightharpoonup> 'sym term"
+type_synonym 'sym function_interpretation = "'sym term \<rightharpoonup> 'sym term"
 
-  fun subterms::"'a term \<Rightarrow> 'a term set" where
-    "subterms (Sym x) = {Sym x}"
-  | "subterms (Fun f as) = insert (Fun f as) (\<Union> (subterms ` (set as)))"
+fun subterms::"'a term \<Rightarrow> 'a term set" where
+  "subterms (Sym x) = {Sym x}"
+| "subterms (Fun f as) = insert (Fun f as) (\<Union> (subterms ` (set as)))"
 
-  lemma term_in_subterms: "x \<in> subterms x"
-    by (cases x) auto
+lemma term_in_subterms: "x \<in> subterms x"
+  by (cases x) auto
+
+lemma args_in_subterms: "set as \<subseteq> subterms (Fun f as)"
+  using term_in_subterms by auto
   
-  lemma args_in_subterms: "set as \<subseteq> subterms (Fun f as)"
-    using term_in_subterms by auto
-    
-  inductive nf_fi::"'a function_interpretation \<Rightarrow> bool"
-        and nf_term::"'a function_interpretation \<Rightarrow> 'a term \<Rightarrow> bool" where
-    "\<lbrakk>\<not>(\<exists>obj. Sym obj \<in> dom fi); 
-        \<forall>(l, r) \<in> Map.graph fi. \<exists>f as. Fun f as = l \<and> list_all (nf_term fi) as \<and> nf_term fi r\<rbrakk> 
-      \<Longrightarrow> nf_fi fi"
-  | "nf_fi fi \<Longrightarrow> nf_term fi (Sym s)"
-  | "\<lbrakk>nf_fi fi; list_all (nf_term fi) as; fi (Fun f as) = None\<rbrakk> 
-      \<Longrightarrow> nf_term fi (Fun f as)"
+inductive nf_fi::"'a function_interpretation \<Rightarrow> bool"
+      and nf_term::"'a function_interpretation \<Rightarrow> 'a term \<Rightarrow> bool" where
+  "\<lbrakk>\<not>(\<exists>obj. Sym obj \<in> dom fi); 
+      \<forall>(l, r) \<in> Map.graph fi. \<exists>f as. Fun f as = l \<and> list_all (nf_term fi) as \<and> nf_term fi r\<rbrakk> 
+    \<Longrightarrow> nf_fi fi"
+| "nf_fi fi \<Longrightarrow> nf_term fi (Sym s)"
+| "\<lbrakk>nf_fi fi; list_all (nf_term fi) as; fi (Fun f as) = None\<rbrakk> 
+    \<Longrightarrow> nf_term fi (Fun f as)"
 
 lemma nf_subterms:
   "nf_term fi x \<longleftrightarrow> (\<forall>t \<in> subterms x. nf_term fi t)"
@@ -48,351 +48,180 @@ next
   qed
 qed
 
-  locale term_eq =
-    fixes fi::"'sym function_interpretation"
-  begin
+locale term_eq =
+  fixes fi::"'sym function_interpretation"
+begin
     
   inductive reduce::"'sym term \<Rightarrow> 'sym term \<Rightarrow> bool" (infix "\<rightarrow>\<^sub>t" 55)where
       refl: "t \<rightarrow>\<^sub>t t"
     | step: "(t1, t2) \<in> Map.graph fi \<Longrightarrow> t1 \<rightarrow>\<^sub>t t2"
     | app: "list_all2 (\<rightarrow>\<^sub>t) as as' \<Longrightarrow> (Fun f as) \<rightarrow>\<^sub>t (Fun f as')"
 
-inductive_cases reduce_appE: "(Fun f as) \<rightarrow>\<^sub>t (Fun f as')"
-
-inductive_cases reduce_funE: "(Fun f as) \<rightarrow>\<^sub>t t"
-
-  definition eq::"'sym term \<Rightarrow> 'sym term \<Rightarrow> bool" (infix "=\<^sub>t" 55) where
-    "x =\<^sub>t y \<equiv> ((\<rightarrow>\<^sub>t)\<^sup>=\<^sup>=) x y"
-
-  end
+  inductive_cases reduce_appE: "(Fun f as) \<rightarrow>\<^sub>t (Fun f as')"
   
-  locale decidable_eq = term_eq fi 
-    for fi::"'sym term \<Rightarrow> 'sym term option" +
-    assumes nf: "nf_fi fi"
-  begin
-    fun normalise_term::"'sym term \<Rightarrow> 'sym term" where
-      "normalise_term (Sym s) = (Sym s)"
-    | "normalise_term (Fun f as) = (
-        let as' = map normalise_term as 
-        in (case (fi (Fun f as')) of
-          Some t  \<Rightarrow> t
-        | None    \<Rightarrow> (Fun f as')
-        )
-      )"
+  inductive_cases reduce_funE: "(Fun f as) \<rightarrow>\<^sub>t t"
+
+  definition term_eq::"'sym term \<Rightarrow> 'sym term \<Rightarrow> bool" (infix "=\<^sub>t" 55) where
+    "term_eq \<equiv> equivclp (\<rightarrow>\<^sub>t)"
+
+  lemma reduce_refl: "(\<rightarrow>\<^sub>t)\<^sup>=\<^sup>= = (\<rightarrow>\<^sub>t)"
+    by (blast intro: refl)
+  
+  lemma reduce_rtrancl_is_trancl: "(\<rightarrow>\<^sub>t)\<^sup>*\<^sup>* = (\<rightarrow>\<^sub>t)\<^sup>+\<^sup>+"
+    apply (rule ext)+
+    subgoal by (auto simp: Nitpick.rtranclp_unfold intro: refl)
+    done
+  
+  find_theorems "?a = ?b \<Longrightarrow> (?a \<Longrightarrow> ?b)"
+
+  lemma reduce_rtranclp_induct': 
+    assumes "reduce\<^sup>*\<^sup>* x y" 
+      "\<And>a b. reduce a b \<Longrightarrow> P a b" 
+      "\<And>a b c. reduce\<^sup>+\<^sup>+ a b \<Longrightarrow> P a b \<Longrightarrow> reduce b c \<Longrightarrow> P a c" 
+    shows "P x y"
+    using assms(1)[simplified reduce_rtrancl_is_trancl]
+    apply (induction rule: tranclp.induct)
+    using assms(2,3) by auto
+
+lemmas reduce_rtranclp_induct = reduce_rtranclp_induct'[rotated, OF reduce.induct, rotated 5]
+thm rtranclp_induct[OF reduce.induct]
+end
+  
+locale decidable_eq = term_eq fi 
+  for fi::"'sym term \<Rightarrow> 'sym term option" +
+  assumes nf: "nf_fi fi"
+begin
+  
+  fun normalise_term::"'sym term \<Rightarrow> 'sym term" where
+    "normalise_term (Sym s) = (Sym s)"
+  | "normalise_term (Fun f as) = (
+      let as' = map normalise_term as 
+      in (case (fi (Fun f as')) of
+        Some t  \<Rightarrow> t
+      | None    \<Rightarrow> (Fun f as')
+      )
+    )"
 
   definition decidable_eq::"'sym term \<Rightarrow> 'sym term \<Rightarrow> bool" where
     "decidable_eq a b \<equiv> (normalise_term a) = (normalise_term b)"
 
-lemma nf_cannot_reduce': 
-  assumes "nf_term fi t"
-  shows "t \<notin> dom fi"
-proof (cases t)
-  case (Sym s)
-  with nf
-  show "t \<notin> dom fi" 
-    apply (cases rule: nf_fi.cases)
-    by simp
-next
-  case (Fun f as)
-  with assms(1)
-  show ?thesis 
-    apply (cases rule: nf_term.cases)
-    by auto
-qed
-
-lemma nf_term_not_fst: "\<not>((x, y) \<in> Map.graph fi \<and> nf_term fi x)"
-  apply (rule notI)
-  apply (erule conjE)
-  apply (drule graph_domD)
-  apply (subst (asm) fst_conv)
-  apply (drule nf_cannot_reduce')
-  by simp
-
-
-lemma nf_cannot_reduce: 
-  assumes "t \<rightarrow>\<^sub>t t'"
-      and "nf_term fi t"
-    shows "t = t'"
-  using assms
-proof (induction t arbitrary: t')
-  case (Sym x)
-  then show ?case 
-  proof (induction "Sym x" t' rule: reduce.induct)
-    case refl
-    then show ?case by simp
+  lemma nf_cannot_reduce': 
+    assumes "nf_term fi t"
+    shows "t \<notin> dom fi"
+  proof (cases t)
+    case (Sym s)
+    with nf
+    show "t \<notin> dom fi" 
+      apply (cases rule: nf_fi.cases)
+      by simp
   next
-    case (step t2)
-    then show ?case using nf_term_not_fst by simp
+    case (Fun f as)
+    with assms(1)
+    show ?thesis 
+      apply (cases rule: nf_term.cases)
+      by auto
   qed
-next
-  case (Fun f as)
-  show ?case
-  proof (cases rule: reduce_funE[OF Fun(2)])
-    case 1
-    then show ?thesis by simp
-  next
-    case 2
-    with Fun(3)
-    show ?thesis using nf_term_not_fst by simp
-  next
-    fix t' as'
-    assume a: "t' = Fun f as'"
-           "list_all2 (\<rightarrow>\<^sub>t) as as'"
-    from Fun(3)
-    have "list_all (nf_term fi) as" by (cases rule: nf_term.cases) auto
-    from a(2) Fun(1) this
-    have "list_all2 (=) as as'"
-      by (induction rule:list_all2_induct) auto
-    from a(1) this[simplified list_all2_eq[symmetric]]
-    show "Fun f as = t'" by blast
-  qed
-qed
 
-lemma unique_reduction:
-  assumes "t1 \<rightarrow>\<^sub>t t2"
-      and "(t1, t2) \<in> Map.graph fi"
-      and "t1 \<rightarrow>\<^sub>t t'"
-    shows "t' = t1 \<or> t' = t2"
-proof (cases t1)
-  case (Sym x)
-  with assms(2)
-  have "False" 
-    apply (cases rule: nf_fi.cases[OF nf])
+  lemma nf_term_not_fst: "\<not>((x, y) \<in> Map.graph fi \<and> nf_term fi x)"
+    apply (rule notI)
+    apply (erule conjE)
     apply (drule graph_domD)
+    apply (subst (asm) fst_conv)
+    apply (drule nf_cannot_reduce')
     by simp
-  then show ?thesis by simp
-next
-  case (Fun f as)
-  show ?thesis
-  proof (rule ccontr)
-    assume "\<not> (t' = t1 \<or> t' = t2)"
-    hence "t' \<noteq> t1" "t' \<noteq> t2" by auto
-    from assms(3, 2) this
-    have "\<exists>as'. list_all2 (\<rightarrow>\<^sub>t) as as' \<and> as \<noteq> as'"
-      unfolding Fun
-    proof (induction "Fun f as" t' arbitrary: t2 rule: reduce.induct)
-      case (refl t)
-      then show ?case by simp
-    next
-      case (trans t t' t'')
-      show ?case 
-      proof (cases "t = Fun f as")
-        case True
-        with trans
-        show ?thesis by simp
-      next
-        case False
-        from \<open>(Fun f as, t'') \<in> Map.graph fi\<close>
-        have "nf_term fi t''" 
-          by (cases rule: nf_fi.cases[OF nf]) auto 
-        have "t \<noteq> t''" 
-        proof
-          assume "t = t''"
-          from nf_cannot_reduce[OF \<open>nf_term fi t''\<close> trans(3)[simplified this]] trans(7)
-          show False by simp
-        qed    
-        from trans(2)[OF trans(5) False this]
-        show ?thesis .
-      qed
-    next
-      case (def t t2')
-      from in_graphD[OF this(1)] in_graphD[OF this(2)] this(4)
-      show ?case by simp
-    next
-      case (app as' t')
-      from this (1)
-      have "list_all2 (\<rightarrow>\<^sub>t) as as'" 
-        by (induction rule: list_all2_induct) auto
-      with app(3)
-      show ?case by blast
-    qed
-    then obtain as' where
-      as': "list_all2 (\<rightarrow>\<^sub>t) as as'"
-      "as \<noteq> as'" by auto 
-    
-    from assms(2)[simplified Fun]
-    have "list_all (nf_term fi) as" 
-    proof (cases rule: nf_fi.cases[OF nf])
-      case (1 fi)
-      with assms(2)[simplified Fun]
-      show ?thesis by fast 
-    qed
-    with as'(1)
-    have "as = as'" 
-    proof (subst list_all2_eq, induction rule: list_all2_induct)
-      case Nil
-      then show ?case by auto
-    next
-      case (Cons x y xs ys)
-      hence "nf_term fi x" by auto
-      with Cons(1)
-      have "x = y" using nf_cannot_reduce by simp
-      then show ?case using Cons by auto
-    qed
-    with as'(2)
-    show False by simp
-  qed
-qed
 
-lemma unique_application:
-  assumes "Fun f as \<rightarrow>\<^sub>t Fun f as'"
-      and "Fun f as \<rightarrow>\<^sub>t t'"
-    shows "t' \<rightarrow>\<^sub>t Fun f as' \<or> Fun f as' \<rightarrow>\<^sub>t t'"
-  using assms(2,1)
-proof (induction rule: reduce.induct)
-  case (refl t)
-  then show ?case sorry
-next
-  case (trans t1 t2 t3)
-  then show ?case sorry
-next
-  case (def t1 t2)
-  then show ?case sorry
-next
-  case (app as as' f)
-  then show ?case sorry
-qed
 
-lemma idk:
-  assumes "t1 \<rightarrow>\<^sub>t t2" 
-      and "t1 \<rightarrow>\<^sub>t t'"
-    shows "t2 \<rightarrow>\<^sub>t t' \<or> t' \<rightarrow>\<^sub>t t2"
-  using assms
-proof (induction arbitrary: t' rule: reduce.induct)
-  case (refl t)
+  thm rtranclp_induct
+  find_theorems name: "rtranclp"
+lemma list_all2_tranclp: "list_all2 (R\<^sup>*\<^sup>*) xs ys \<Longrightarrow> reflp R \<Longrightarrow> (list_all2 R)\<^sup>*\<^sup>* xs ys"
+proof (induction rule: list_all2_induct)
+  case Nil
   then show ?case by simp
 next
-  case (trans t t2 t3)
-  then consider "t2 \<rightarrow>\<^sub>t t'" | "t' \<rightarrow>\<^sub>t t2" by auto
-  then show ?case 
-  proof (cases)
-    case 1
-    from trans.IH(2)[OF this]
-    show ?thesis .
-  next
-    case 2
-    from reduce.trans[OF this \<open>t2 \<rightarrow>\<^sub>t t3\<close>]
-    show ?thesis by simp
-  qed
-next
-  case (def t1 t2)
-  from unique_reduction def(1)[THEN reduce.def] def
-  consider "t' = t1" | "t' = t2" by blast
+  case (Cons x y xs ys)
   then show ?case
-  proof (cases)
-    case 1
-    from def 
-    have "t1 \<rightarrow>\<^sub>t t2" using reduce.def by auto 
-    with 1
-    show ?thesis by simp
+  proof (induction rule: rtranclp.induct)
+    case (rtrancl_refl a)
+    then show ?case sorry
   next
-    case 2
-    then show ?thesis using refl by auto
+    case (rtrancl_into_rtrancl a b c)
+    then show ?case sorry
   qed
-next
-  case (app as as' f)
-  have "list_all2 (\<lambda>x1 x2. x1 \<rightarrow>\<^sub>t x2) as as'" using app(1)
-    by (induction rule: list_all2_induct) auto
-  then
-  have "Fun f as \<rightarrow>\<^sub>t Fun f as'" using reduce.app by simp
-  with app(2, 1) this
-  show ?case 
-  proof (induction "Fun f as" t' rule: reduce.induct)
-    case refl
-    then show ?case by simp
+qed
+
+  lemma nf_cannot_reduce: 
+    assumes "t \<rightarrow>\<^sub>t t'"
+        and "nf_term fi t"
+      shows "t = t'"
+    using assms
+  proof (induction t arbitrary: t')
+    case (Sym x)
+    then show ?case 
+    proof (induction "Sym x" t' rule: reduce.induct)
+      case refl
+      then show ?case by simp
+    next
+      case (step t2)
+      then show ?case using nf_term_not_fst by simp
+    qed
   next
-    case (trans t2 t3)
+    case (Fun f as)
     show ?case
-    proof (cases "t2 = Fun f as")
-      case True
-      with trans 
-      show ?thesis by auto
+    proof (cases rule: reduce_funE[OF Fun(2)])
+      case 1
+      then show ?thesis by simp
     next
-      case False
-      from trans
-      have "Fun f as' \<rightarrow>\<^sub>t t2 \<or> t2 \<rightarrow>\<^sub>t Fun f as'" by auto
-      with trans(1,3,4,5,6,7) app
-      show ?thesis 
+      case 2
+      with Fun(3)
+      show ?thesis using nf_term_not_fst by simp
+    next
+      fix t' as'
+      assume a: "t' = Fun f as'"
+             "list_all2 (\<rightarrow>\<^sub>t) as as'"
+      from Fun(3)
+      have "list_all (nf_term fi) as" by (cases rule: nf_term.cases) auto
+      from a(2) Fun(1) this
+      have "list_all2 (=) as as'"
+        by (induction rule:list_all2_induct) auto
+      from a(1) this[simplified list_all2_eq[symmetric]]
+      show "Fun f as = t'" by blast
     qed
-  next
-    case (def t2)
-    then show ?case sorry
-  next
-    case (app as')
-    then show ?case sorry
   qed
-qed
 
-lemma nf_reachable: 
-  assumes "t \<rightarrow>\<^sub>t t'" "nf_term fi t'"
-          "t \<rightarrow>\<^sub>t t''"
-    shows "t'' \<rightarrow>\<^sub>t t'"
-  using assms
-proof (induction arbitrary: t'' rule: reduce.induct)
-  case (refl t)
-  then show ?case using nf_cannot_reduce by blast
+  find_theorems name: "list_all*"
+
+lemma normalise_in_trans_reduce: "(\<rightarrow>\<^sub>t)\<^sup>*\<^sup>* t (normalise_term t)"
+proof (induction t)
+  case (Sym x)
+  then show ?case by simp
 next
-  case (trans t1 t2 t3)
-  with 
-  show ?case
-  proof (cases "t2 = t3")
-    case True
-    then show ?thesis using trans by simp
-  next
-    case False
+  case (Fun f as)
+  have 1: "list_all2 ((\<rightarrow>\<^sub>t)\<^sup>*\<^sup>*) as (map normalise_term as)" 
+    using Fun.IH by (induction as, auto)
+  hence "((list_all2 (\<rightarrow>\<^sub>t))\<^sup>*\<^sup>*) as (map normalise_term as)"
+    apply (induction rule: list_all2_induct)
+     apply simp
+    
+  show ?case 
+  proof (cases "fi (Fun f (map normalise_term as))")
+    case None
+    then have 2: "normalise_term (Fun f as) = (Fun f (map normalise_term as))" by simp
+
     show ?thesis 
-    proof (cases "t'' = t3")
-      case True
-      then show ?thesis using refl by simp
-    next
-      case False
-      show ?thesis 
-      proof (cases "t'' = t2")
-        case True
-        then show ?thesis using trans by simp
-      next
-        case False
-        with \<open>t'' \<noteq> t3\<close> \<open>t2 \<noteq> t3\<close>
-        show ?thesis using trans 
-      qed
-    qed
+      unfolding 2
+    proof (induction rule: rtranclp.induct)
+  next
+    case (Some a)
+    then show ?thesis sorry
   qed
-next
-  case (def t1 t2)
-  then show ?case sorry
-next
-  case (app as as' f)
-  then show ?case sorry
-qed
-
-
-lemma nf_unique:
-  assumes 1: "t \<rightarrow>\<^sub>t t'" "nf_term fi t'"
-      and 2: "t \<rightarrow>\<^sub>t t''" "nf_term fi t''"
-    shows "t' = t''"
-  using assms
-proof (induction arbitrary: t'' rule: reduce.induct)
-  case (refl t)
-  then show ?case using nf_cannot_reduce by simp
-next
-  case (trans t1 t2 t3)
-  from nf_reachable[OF \<open>t1 \<rightarrow>\<^sub>t t''\<close> \<open>nf_term fi t''\<close> \<open>t1 \<rightarrow>\<^sub>t t2\<close>]
-  have "t2 \<rightarrow>\<^sub>t t''" by auto
-  with trans.IH(2) trans.prems
-  show ?case by simp 
-next
-  case (def t1 t2)
-  then show ?case sorry
-next
-  case (app as as' f)
-  then show ?case sorry
 qed
 
   
   lemma normalise_nf: "nf_term fi (normalise_term t)"
     sorry
-  theorem decidable_eq_correct: "eq a b \<longleftrightarrow> decidable_eq a b"
+  
+  theorem decidable_eq_correct: "term_eq a b \<longleftrightarrow> decidable_eq a b"
     sorry
-  end
+end
   
 end
